update compile_top_labels

compiler/proofs/compilerProofScript.sml
@@ -118,6 +118,27 @@ val evaluate_prompt_i1_success_globals = store_thm("evaluate_prompt_i1_success_g
     EVERY IS_SOME new_genv``,
   rw[evaluate_prompt_i1_cases] >> rw[EVERY_MAP])
 
+val local_labels_def = Define`
+  local_labels code = FILTER ($~ o inst_uses_label VfromListLab) code`
+
+val local_labels_append = store_thm("local_labels_append[simp]",
+  ``∀l1 l2. local_labels (l1 ++ l2) = local_labels l1 ++ local_labels l2``,
+  rw[local_labels_def,FILTER_APPEND])
+
+val local_labels_reverse = store_thm("local_labels_reverse[simp]",
+  ``∀l1. local_labels (REVERSE l1) = REVERSE (local_labels l1)``,
+  rw[local_labels_def,FILTER_REVERSE])
+
+val FILTER_is_Label_local_labels = store_thm("FILTER_is_Label_local_labels[simp]",
+  ``∀code. FILTER is_Label (local_labels code) = FILTER is_Label code``,
+  rw[local_labels_def,FILTER_FILTER] >>
+  rw[FILTER_EQ,is_Label_rwt,EQ_IMP_THM] >>
+  rw[])
+
+val MEM_Label_local_labels = store_thm("MEM_Label_local_labels[simp]",
+  ``∀l c. MEM (Label l) (local_labels c) ⇔ MEM (Label l) c``,
+  rw[local_labels_def,MEM_FILTER])
+
 (* misc *)
 
 val code_env_cd_append = store_thm("code_env_cd_append",
@@ -1093,8 +1114,8 @@ val compile_Cexp_thm = store_thm("compile_Cexp_thm",
     ⇒
     let cs' = compile_Cexp renv rsz cs exp in
     ∃c0 code. cs'.out = REVERSE code ++ REVERSE c0 ++ cs.out ∧
-    between_labels (FILTER ($~ o inst_uses_label VfromListLab) (c0++code)) cs.next_label cs'.next_label ∧
-    code_labels_ok (FILTER ($~ o inst_uses_label VfromListLab) (c0++code)) ∧
+    between_labels (local_labels (c0++code)) cs.next_label cs'.next_label ∧
+    code_labels_ok (local_labels (c0++code)) ∧
     ∀s env res rd csz bs bc0 bc00.
       Cevaluate s env exp res
     ∧ closed_vlabs env s bc0
@@ -1125,6 +1146,7 @@ val compile_Cexp_thm = store_thm("compile_Cexp_thm",
     | Rerr Rtimeout_error =>
       ∃bs'. bc_next^* bs bs' ∧ bs'.clock = SOME 0 ∧ bc_fetch bs' = SOME Tick ∧ bs'.output = bs.output
     | _ => T``,
+  REWRITE_TAC[local_labels_def] >>
   rw[compile_Cexp_def] >>
   qspecl_then[`LENGTH renv`,`cs.next_label`,`exp`]mp_tac (CONJUNCT1 label_closures_thm) >>
   simp[] >> strip_tac >>
@@ -1544,8 +1566,8 @@ val compile_top_labels = store_thm("compile_top_labels",
       FV_top top ⊆ global_dom rs.globals_env
       ⇒
       (FST(SND(compile_top types rs top))).rnext_label = (FST(compile_top types rs top)).rnext_label ∧
-      between_labels (SND(SND(compile_top types rs top))) rs.rnext_label (FST(compile_top types rs top)).rnext_label ∧
-      code_labels_ok (SND(SND(compile_top types rs top)))``,
+      between_labels (local_labels (SND(SND(compile_top types rs top)))) rs.rnext_label (FST(compile_top types rs top)).rnext_label ∧
+      code_labels_ok (local_labels (SND(SND(compile_top types rs top))))``,
    simp[compile_top_def,UNCURRY,pair_CASE_def] >>
    rpt gen_tac >> strip_tac >>
    specl_args_of_then``compile_Cexp``compile_Cexp_thm mp_tac >>
@@ -1593,7 +1615,9 @@ val compile_top_labels = store_thm("compile_top_labels",
    match_mp_tac code_labels_ok_append >>
    simp[code_labels_ok_REVERSE] >>
    REWRITE_TAC[GSYM REVERSE_APPEND] >>
-   simp[code_labels_ok_REVERSE] )
+   simp[code_labels_ok_REVERSE] >>
+   fs[local_labels_def,code_labels_ok_def,uses_label_thm,EXISTS_MEM,MEM_FILTER,PULL_EXISTS] >>
+   metis_tac[])
 
 val tac1 =
   simp[store_to_exh_def] >>
